Add Unknown as a terminating instruction

attic/BasicBlocks.thy
@@ -120,6 +120,7 @@ fun aux_basic_block :: "pos_inst list \<Rightarrow> pos_inst list \<Rightarrow> 
   | Misc RETURN \<Rightarrow>(bl_pt, block @ [i], No) # ( aux_basic_block tl1 [])
   | Misc SUICIDE \<Rightarrow>(bl_pt, block @ [i], No) # ( aux_basic_block tl1 [])
   | Misc STOP \<Rightarrow>(bl_pt, block @ [i], No) # ( aux_basic_block tl1 [])
+  | Unknown a \<Rightarrow> (bl_pt, block @ [i], No) # ( aux_basic_block tl1 [])
   | _ \<Rightarrow> aux_basic_block tl1 (block@[i])))"
 declare aux_basic_block.simps[simp del]
 
@@ -142,6 +143,7 @@ fun reg_inst :: "inst \<Rightarrow> bool" where
 |"reg_inst (Misc RETURN) = False"
 |"reg_inst (Misc SUICIDE) = False"
 |"reg_inst (Misc _) = True"
+|"reg_inst (Unknown a) = False"
 |"reg_inst _ = True"
 
 definition reg_block :: "pos_inst list \<Rightarrow> bool" where
@@ -162,7 +164,7 @@ fun seq_block :: "pos_inst list \<Rightarrow> bool" where
 declare seq_block.simps[simp del]
 
 definition last_no::"pos_inst list \<Rightarrow> bool" where
-"last_no insts == snd (last insts) \<in> {Misc STOP, Misc RETURN, Misc SUICIDE}"
+"last_no insts == snd (last insts) \<in> {Misc STOP, Misc RETURN, Misc SUICIDE} \<or> (\<exists>a. snd (last insts) = Unknown a)"
 
 definition wf_blocks:: "basic_blocks \<Rightarrow> bool" where
 "wf_blocks c == 
@@ -196,6 +198,7 @@ apply(induction insts arbitrary: block n j i t xs b)
  apply(clarsimp)
 apply(simp add: aux_basic_block.simps Let_def)
 apply(simp split: inst.splits add: inst_size_def inst_code.simps)
+  apply(clarsimp simp add: block_pt_def split: list.splits)
  apply(clarsimp simp add: block_pt_def split: pc_inst.splits list.splits if_splits)
 apply(clarsimp simp add: block_pt_def split: misc_inst.splits list.splits)
 done
@@ -224,6 +227,8 @@ apply(subgoal_tac "(n, b, t) \<in> set
  apply(drule subst[OF aux_basic_block.simps(3)])
  apply(simp add: Let_def)
   apply(clarsimp split: inst.splits simp add: inst_size_def inst_code.simps)
+   apply(erule disjE, rule_tac x="(a,Unknown x1) # insts" in exI, rule_tac x=block in exI,
+				simp add: aux_basic_block.simps Let_def, fastforce)
   apply(simp split: pc_inst.splits if_splits add: inst_size_def inst_code.simps;
 				erule disjE, rule_tac x="(a,Pc x9) # insts" in exI, rule_tac x=block in exI,
 				simp add: aux_basic_block.simps Let_def, fastforce)
@@ -467,7 +472,8 @@ apply(induction c arbitrary: b)
 apply(simp add: aux_basic_block.simps Let_def)
 apply(case_tac "reg_inst (snd a) \<and> snd a \<noteq> Pc JUMPDEST")
  apply(simp split: reg_inst_splits)
- apply(drule conjunct1; rule conjI; rule allI; clarify; rule conjI)
+ apply(drule conjunct1; rule conjI, clarsimp)
+ apply(rule conjI; rule allI; clarify; rule conjI)
   apply(clarsimp)+
  apply(rule conjI; clarsimp)
 apply(case_tac "snd a = Pc JUMPDEST"; clarsimp)
